backend/Tailcallproof.v
@@ -221,26 +221,14 @@ Proof.
   intros. apply match_transform_program_contextual; auto.
 Qed.
 
-Definition match_pol (prog: program) := Policy.match_pol_gen (fun cunit f tf => tf = transf_fundef (compenv_program cunit) f) prog.
-
 Section PRESERVATION.
 
 Variable prog tprog: program.
 Hypothesis TRANSL: match_prog prog tprog.
 
-Variable pol: policy.
-Variable tpol: policy.
-Hypothesis TRANSPOL: match_pol prog pol tpol.
 
 Let ge := Genv.globalenv prog.
 Let tge := Genv.globalenv tprog.
-
-Lemma linkorder_policy:
-  forall cunit, linkorder cunit prog ->
-           Policy.match_pol_gen (fun cunit f tf => tf = transf_fundef (compenv_program cunit) f) prog pol tpol ->
-           Policy.match_pol_gen (fun cunit f tf => tf = transf_fundef (compenv_program cunit) f) cunit pol tpol.
-Proof.
-Admitted.
 
 Lemma symbols_preserved:
   forall (s: ident), Genv.find_symbol tge s = Genv.find_symbol ge s.
@@ -501,9 +489,9 @@ Ltac EliminatedInstr :=
   of the ``option'' kind. *)
 
 Lemma transf_step_correct:
-  forall s1 t s2, step pol ge s1 t s2 ->
+  forall s1 t s2, step ge s1 t s2 ->
   forall s1' (MS: match_states s1 s1'),
-  (exists s2', step tpol tge s1' t s2' /\ match_states s2 s2')
+  (exists s2', step tge s1' t s2' /\ match_states s2 s2')
   \/ (measure s2 < measure s1 /\ t = E0 /\ match_states s2 s1')%nat.
 Proof.
   induction 1; intros; inv MS; EliminatedInstr.
@@ -575,11 +563,9 @@ Proof.
   { change (fn_comp _) with (comp_of (transf_function ce f)).
     now rewrite comp_transl, comp_transl. }
   { now rewrite <- E. }
-  eapply linkorder_policy; eauto.
-  rewrite <- E; auto.
   constructor. eapply match_stackframes_tail; eauto.
     apply (cenv_compat_linkorder _ _ _ ORDER (compenv_program_compat _)).
-  { red. now rewrite Efd, ALLOWED0. }
+  { red. now rewrite Efd, ALLOWED. }
   apply regs_lessdef_regs; auto.
   eapply Mem.free_right_extends; eauto.
   rewrite stacksize_preserved. rewrite H7. intros. omegaContradiction.
@@ -587,8 +573,6 @@ Proof.
   left. exists (Callstate (Stackframe res (transf_function ce f) (Vptr sp0 Ptrofs.zero) pc' rs' :: s')
                           (transf_fundef (compenv_program cu) fd) (rs'##args) m'); split.
   eapply exec_Icall; eauto. apply sig_preserved.
-  eapply linkorder_policy; eauto.
-  rewrite <- E; auto.
   constructor. constructor; auto.
     apply (cenv_compat_linkorder _ _ _ ORDER (compenv_program_compat _)).
   { easy. }
@@ -604,8 +588,6 @@ Proof.
   eapply exec_Itailcall; eauto. apply sig_preserved.
     now rewrite comp_transl, COMP.
   { now rewrite Ef in ALLOWED. }
-  eapply linkorder_policy; eauto.
-  rewrite Ef in ALLOWED'; auto.
   rewrite stacksize_preserved; auto.
   constructor. auto.
     apply (cenv_compat_linkorder _ _ _ ORDER (compenv_program_compat _)).
@@ -621,11 +603,8 @@ Proof.
   left. exists (State s' (transf_function ce f) (Vptr sp0 Ptrofs.zero) pc' (regmap_setres res v' rs') m'1); split.
   eapply exec_Ibuiltin; eauto.
   eapply eval_builtin_args_preserved with (ge1 := ge); eauto. exact symbols_preserved.
-  eapply TRANSPOL with (f := External ef); eauto.
   rewrite comp_transf_function; eauto.
   eapply external_call_symbols_preserved; eauto. apply senv_preserved.
-  change (fn_comp (transf_function _ _)) with (comp_of (transf_function ce f)).
-  now rewrite comp_transl.
   econstructor; eauto. apply set_res_lessdef; auto.
 
 
@@ -741,7 +720,7 @@ Qed.
   follows. *)
 
 Theorem transf_program_correct:
-  forward_simulation (RTL.semantics pol prog) (RTL.semantics tpol tprog).
+  forward_simulation (RTL.semantics prog) (RTL.semantics tprog).
 Proof.
   eapply forward_simulation_opt with (measure := measure); eauto.
   apply senv_preserved.
